Iris/Iris/ProgramLogic/TotalLifting.lean
@@ -29,10 +29,7 @@ theorem twp_lift_step (h : toVal e₁ = none) :
         stateInterp σ₂ (ns + 1) obs (nt + eₜ.length) ∗
         WP e₂ @ s; E [{ Φ }] ∗
         [∗list] ef ∈ eₜ, WP ef @ s; ⊤ [{ ι.forkPost }])
-    ⊢ WP e₁ @ s; E [{ Φ }] := by
-  rw [twp.unfold.to_eq]
-  simp only [twp.pre, h]
-  exact .rfl
+    ⊢ WP e₁ @ s; E [{ Φ }] := by rw [twp.unfold.to_eq, twp.pre, h]
 
 theorem twp_lift_step_no_fork (h : toVal e₁ = none) :
     (∀ σ₁ ns obs nt, stateInterp σ₁ ns obs nt ={E,∅}=∗
@@ -42,17 +39,13 @@ theorem twp_lift_step_no_fork (h : toVal e₁ = none) :
         stateInterp σ₂ (ns + 1) obs nt ∗
         WP e₂ @ s; E [{ Φ }])
     ⊢ WP e₁ @ s; E [{ Φ }] := by
-  iintro H
-  iapply twp_lift_step h
-  iintro %σ₁ %ns %obs %nt Hσ
+  refine .trans ?_ <| twp_lift_step h
+  iintro H %σ₁ %ns %obs %nt Hσ
   imod H $$ Hσ with ⟨%Hred, H⟩
-  imodintro
   iframe %Hred
-  iintro %κ %e₂ %σ₂ %eₜ %Hstep
-  imod H $$ %κ %e₂ %σ₂ %eₜ %Hstep with ⟨%hκ, %heₜ, Hσ, Hwp⟩
-  subst heₜ
-  imodintro
-  simp only [List.length_nil, Nat.add_zero, Algebra.BigOpL.bigOpL_nil]
+  iintro !> %κ %e₂ %σ₂ %eₜ Hstep
+  imod H $$ Hstep with ⟨%hκ, %heₜ, Hσ, Hwp⟩
+  simp only [heₜ, List.length_nil, Nat.add_zero, Algebra.BigOpL.bigOpL_nil, BI.sep_emp.to_eq]
   iframe %hκ Hσ Hwp
 
 @[rocq_alias twp_lift_atomic_step]
@@ -65,23 +58,17 @@ theorem twp_lift_atomic_step (h : toVal e₁ = none) :
         (∃ v, ⌜toVal e₂ = some v⌝ ∧ Φ v) ∗
         [∗list] ef ∈ eₜ, WP ef @ s; ⊤ [{ ι.forkPost }])
     ⊢ WP e₁ @ s; E [{ Φ }] := by
-  iintro H
-  iapply twp_lift_step h
-  iintro %σ₁ %ns %obs %nt Hσ
+  refine .trans ?_ <| twp_lift_step h
+  iintro H %σ₁ %ns %obs %nt Hσ
   imod H $$ Hσ with ⟨%Hred, H⟩
   iapply fupd_mask_intro Std.LawfulSet.empty_subset
   iintro Hclose
-  isplit
-  · ipureintro
-    exact Hred
-  · iintro %κ %e₂ %σ₂ %eₜ %Hstep
-    imod Hclose with -
-    imod H $$ %κ %e₂ %σ₂ %eₜ %Hstep with
-      ⟨%hκ, Hσ, ⟨%v, %hval, HΦ⟩, Hefs⟩
-    imodintro
-    iframe %hκ Hσ Hefs
-    iapply twp.value (ToVal.coe_of_toVal_eq_some hval).symm
-    iexact HΦ
+  iframe %Hred
+  iintro %κ %e₂ %σ₂ %eₜ Hstep
+  imod Hclose with -
+  imod H $$ Hstep with ⟨%hκ, Hσ, ⟨%v, %hval, HΦ⟩, Hefs⟩
+  iframe %hκ Hσ Hefs
+  iapply twp.value (ToVal.coe_of_toVal_eq_some hval).symm $$ HΦ
 
 theorem twp_lift_atomic_step_no_fork (h : toVal e₁ = none) :
     (∀ σ₁ ns obs nt, stateInterp σ₁ ns obs nt ={E}=∗
@@ -91,18 +78,13 @@ theorem twp_lift_atomic_step_no_fork (h : toVal e₁ = none) :
         stateInterp σ₂ (ns + 1) obs nt ∗
         ∃ v, ⌜toVal e₂ = some v⌝ ∧ Φ v)
     ⊢ WP e₁ @ s; E [{ Φ }] := by
-  iintro H
-  iapply twp_lift_atomic_step h
-  iintro %σ₁ %ns %obs %nt Hσ
+  refine .trans ?_ <| twp_lift_atomic_step h
+  iintro H %σ₁ %ns %obs %nt Hσ
   imod H $$ Hσ with ⟨%Hred, H⟩
-  imodintro
   iframe %Hred
-  iintro %κ %e₂ %σ₂ %eₜ %Hstep
-  imod H $$ %κ %e₂ %σ₂ %eₜ %Hstep with
-    ⟨%hκ, %heₜ, Hσ, Hval⟩
-  subst heₜ
-  imodintro
-  simp only [List.length_nil, Nat.add_zero, Algebra.BigOpL.bigOpL_nil]
+  iintro !> %κ %e₂ %σ₂ %eₜ Hstep
+  imod H $$ Hstep with ⟨%hκ, %heₜ, Hσ, Hval⟩
+  simp only [heₜ, List.length_nil, Nat.add_zero, Algebra.BigOpL.bigOpL_nil, BI.sep_emp.to_eq]
   iframe %hκ Hσ Hval
 
 @[rocq_alias twp_lift_pure_step_no_fork]
@@ -115,33 +97,19 @@ theorem twp_lift_pure_step_no_fork [Inhabited State]
       ⌜(e₁, σ) -<κ>-> (e₂', σ, eₜ)⌝ -∗
       WP e₂' @ s; E [{ Φ }])
     ⊢ WP e₁ @ s; E [{ Φ }] := by
-  iintro H
-  have hnone : toVal e₁ = none :=
-    Language.toVal_none_of_reducible
-      (Language.reducible_of_reducibleNoObs (Hsafe default))
-  iapply twp_lift_step_no_fork hnone
-  iintro %σ₁ %ns %obs %nt Hσ
-  imod H with H
+  refine .trans ?_ <| twp_lift_step_no_fork (toVal_none_of_reducible <| reducible_of_reducibleNoObs (Hsafe default))
+  iintro H %σ₁ %ns %obs %nt Hσ
+  imod H
   iapply fupd_mask_intro Std.LawfulSet.empty_subset
   iintro Hclose
-  isplit
-  · ipureintro
-    cases s
-    · exact Hsafe σ₁
-    · trivial
+  isplitr
+  · exact BI.pure_intro (by grind [cases Stuckness])
   · iintro %κ %e₂' %σ₂ %eₜ %Hstep
-    obtain ⟨rfl, rfl, rfl⟩ := Hpure _ _ _ _ _ Hstep
+    obtain ⟨hκ, rfl, heₜ⟩ := Hpure _ _ _ _ _ Hstep
     imod ι.stateInterp_mono σ₂ ns obs nt $$ Hσ with Hσ
     imod Hclose
-    imodintro
-    iframe Hσ
-    isplit
-    · ipureintro
-      exact rfl
-    · isplit
-      · ipureintro
-        exact rfl
-      · iapply H $$ %([] : List Obs) %e₂' %([] : List Expr) %σ₂ %Hstep
+    iframe %hκ %heₜ Hσ
+    iapply H $$ %κ %e₂' %eₜ %σ₂ %Hstep
 
 @[rocq_alias twp_lift_pure_det_step_no_fork]
 theorem twp_lift_pure_det_step_no_fork [Inhabited State]
@@ -150,37 +118,16 @@ theorem twp_lift_pure_det_step_no_fork [Inhabited State]
       (e₁, σ₁) -<κ>-> (e₂', σ₂, eₜ) →
       κ = [] ∧ σ₂ = σ₁ ∧ e₂' = e₂ ∧ eₜ = []) :
     (|={E}=> WP e₂ @ s; E [{ Φ }]) ⊢ WP e₁ @ s; E [{ Φ }] := by
-  iintro Hwp
-  iapply twp_lift_pure_step_no_fork Hsafe ?_
-  · intro σ₁ κ e₂' σ₂ eₜ Hstep
-    obtain ⟨hκ, hσ, _, heₜ⟩ := Hpure _ _ _ _ _ Hstep
-    exact ⟨hκ, hσ, heₜ⟩
-  · imod Hwp with Hwp
-    imodintro
-    iintro %κ %e₂' %eₜ %σ %Hstep
-    obtain ⟨_, _, he₂, _⟩ := Hpure _ _ _ _ _ Hstep
-    subst e₂'
-    iexact Hwp
+  refine (BIFUpdate.mono ?_).trans <| twp_lift_pure_step_no_fork Hsafe (by grind only)
+  iintro Hwp %κ %e₂' %eₜ %σ %Hstep
+  exact (Hpure _ _ _ _ _ Hstep).2.2.1 ▸ .rfl
 
 @[rocq_alias twp_pure_step]
 theorem twp_pure_step [Inhabited State]
     (Hexec : PureExec φ n e₁ e₂) (Hφ : φ) :
-    WP e₂ @ s; E [{ Φ }] ⊢ WP e₁ @ s; E [{ Φ }] := by
-  replace Hexec := Hexec.pureExec Hφ
-  iinduction Hexec using Relation.Iterate.head_induction_on with
-  | rfl =>
-      iintro Hwp
-      iexact Hwp
-  | @head n e₁ e₃ _ _ IH =>
-      iintro Hwp
-      obtain ⟨Hsafe, Hdet⟩ := ‹e₁ -ᵖ-> e₃›
-      iapply twp_lift_pure_det_step_no_fork Hsafe ?_
-      · intro σ₁ κ e₂' σ₂ eₜ Hstep
-        obtain ⟨hκ, hσ, he, heₜ⟩ := Hdet Hstep
-        exact ⟨hκ, hσ.symm, he.symm, heₜ⟩
-      · imodintro
-        iapply IH
-        iexact Hwp
+    WP e₂ @ s; E [{ Φ }] ⊢ WP e₁ @ s; E [{ Φ }] := (Hexec.pureExec Hφ).head_induction_on
+      (motive := fun _ e _ => WP e₂ @ s; E [{ Φ }] ⊢ WP e @ s; E [{ Φ }]) .rfl fun e₃ Hstep _ IH =>
+    (IH.trans fupd_intro).trans <| twp_lift_pure_det_step_no_fork (e₂ := e₃) Hstep.1 (by grind only [Hstep.2])
 
 end
 end Iris.ProgramLogic
